\subsection{Wave Equation}
\subsubsection{Separation of Variables}
The general form of the wave equation is
$$\frac{\partial^2 u}{\partial t^2}=c^2\frac{\partial^2u}{\partial x^2}$$
In order to find a solution, we will again require two boundary conditions as well as two initial conditions: $u(x,0)$ and $u_t(x,0)$ normally.\\
We can use many of the same techniques to solve the wave equation as we did to solve the heat equation.\\
Ex:
\begin{align*}
    &u_{tt}=u_{xx},\ 0\leq x\leq \pi,\ t\geq 0\\
    &u_x(0,t)=u_x(\pi,t)=0\\
    &u(x,0)=f(x)=5\cos x\\
    &u_t(x,0)=g(x)=1-2\cos(2x)
\end{align*}
We will start by using separation of variables and finding the eigenvalues and eigenfunctions, the same as was done with the heat equation.
\begin{align*}
    &u(x,t)=X(x)T(t)\\
    &XT''=X''T\Ra \frac{T''}{T}=\frac{X''}{X}=-\lambda\\
    &X''+\lambda X=0,\ X'(0)=X'(\pi)=0\\
    &\leadsto \lambda_0=0,\ \lambda_n=\brround{\frac{n\pi}{L}}^2=n^2\\
    &X_0=1,\ X_n=\cos(nx)\\
    &T_n''+\lambda_n T_n=0\\
    &\lambda_0=0:\ T_0''=0\Ra T_0=A_0+B_0t\\
    &\lambda_n=n^2:\ T_n''+n^2T_n=0\Ra T_n=A_n\cos(nt)+B_n\sin(nt)\\
    &u(x,t)=A_0+B_0t+\sum_{n=1}^\infty\cos(nx)\brround{A_n\cos(nt)+B_n\sin(nt)}\\
    &u_t(x,t)=B_0+\sum_{n=1}^\infty\cos(nx)(n)\brround{-A_n\sin(nt)+B_n\cos(nt)}
\end{align*}
Now we can use our two initial conditions to solve for $A_0,A_n,B_0,B_n$
\begin{align*}
    &u(x,0)=5\cos x=A_0+\sum_{n=1}^\infty A_n\cos(nx)\\
    &\Ra A_0=0,\ A_n=5\delta_{1,n}\\
    &u_t(x,0)=1-2\cos(2x)=B_0+\sum_{n=1}^\infty(B_n n)\cos(nx)\\
    &\Ra B_0=1,\ B_n=-\delta_{n,2}\\
    &u(x,t)=t+\sum_{n=1}^\infty\brround{5\delta_{1,n}\cos(nt)-\delta_{2,n}\sin(nt)}\cos(nx)\\
    &u(x,t)=t+5\cos t\cos x-\sin(2t)\cos(2x)
\end{align*}
The separation of variables method will work for any of the following forms:
\begin{align*}
    &u_{tt}=c^2u_{xx}\\
    &u_{tt}=c^2u_{xx}-\gamma u\\
    &u_{tt}=c^2u_{xx}-\gamma(t)u\\
    &u_{tt}=c^2u_{xx}-\gamma u_t+\eta(t) u
\end{align*}
Ex2:
\begin{align*}
    &u_{tt}=u_{xx}-\gamma u,\ 0<x<1,\ t>0\\
    &u(0,t)=u(1,t)=0\\
    &u(x,0)=0,\ u_t(x,0)=g(x)\\
    &u(x,t)=X(x)T(t)\\
    &\frac{T''}{T}=\frac{X''}{X}-\gamma\Ra \frac{T''}{T}+\gamma=\frac{X''}{X}=-\lambda
\end{align*}
Dirichlet boundary conditions
\begin{align*}
    &\lambda_n=(n\pi)^2\\
    &X_n=\sin(n\pi x)\\
    &T_n''+T_n(\gamma+\lambda)=T_n''+T_n(\gamma+(n\pi)^2)=0\\
    &\text{assuming }\gamma\geq0,\ \mu_n=\sqrt{\gamma+(n\pi)^2}\\
    &T_n=A_n\cos(\mu_nt)+B_n\sin(\mu_nt)\\
    &u(x,t)=\sum_{n=1}^\infty\sin(n\pi x)\brround{A_n\cos(\mu_nt)+B_n\sin(\mu_nt)}\\
    &u_t(x,t)=\sum_{n=1}^\infty\sin(n\pi x)\brround{-A_n\mu_n\sin(\mu_nt)+B_n\mu_n\cos(\mu_nt)}\\
    &u(x,0)=\sum_{n=1}^\infty A_n\sin(n\pi x)=0\Ra A_n=0\\
    &u_t(x,0)=\sum_{n=1}^\infty B_n\mu_n\sin(n\pi x)=g(x)\\
    &B_n\mu_n=2\int_0^1g(x)\sin(n\pi x)dx\Ra B_n=\frac{2}{\mu_n}\int_0^1g(x)\sin(n\pi x)dx\\
    &u(x,t)=\sum_{n=1}^\infty B_n\sin(n\pi x)\sin(t\sqrt{\gamma+(n\pi)^2})=\sum_{n=1}^\infty\frac{2\sin(n\pi x)\sin(t\sqrt{\gamma+(n\pi)^2})}{\sqrt{\gamma+(n\pi)^2}}\int_0^1g(x)\sin(n\pi x)dx
\end{align*}
We can also use the same methods of dealing with inhomogeneous equations for the wave equation as we did with the heat equation.\\
Ex3:
\begin{align*}
    &u_{tt}=u_{xx},\ t>0,\ 0\leq x\leq 1\\
    &u(0,t)=0,\ u(1,t)=1\\
    &u(x,0)=\sin(\pi x)+x,\ u_t(x,0)=\sin(3\pi x)
\end{align*}
Steady state solution:
\begin{align*}
    &u(x,t)=w(x)+v(x,t)\\
    &w_{tt}=0=w_{xx}\Ra w(x)=Ax+B\\
    &w(0)=0\Ra B=0\\
    &w(1)=1=A\\
    &w(x)=x\\
    &w_{tt}+v_{tt}=w_{xx}+v_{xx}\Ra v_{tt}=v_{xx}\\
    &w(0)+v(0)=0\Ra v(0)=0\\
    &w(1)+v(1)=1\Ra v(1)=0\\
    &w(x)+v(x,0)=x+v(x,0)=\sin(\pi x)+x\Ra v(x,0)=\sin(\pi x)\\
    &w_t(x)+v_t(x,0)=\sin(3\pi x)\Ra v_t(x,0)=\sin(3\pi x)
\end{align*}
Separation of variables:\\
Dirichlet BCs
\begin{align*}
    &\lambda_n=(n\pi)^2\\
    &X_n=\sin(n\pi x)\\
    &T_n''+\lambda_nT_n=T_n''+(n\pi)^2T_n'=0\\
    &\Ra T_n=A_n\cos(n\pi t)+B_n\sin(n\pi t)\\
    &v(x,t)=\sum_{n=1}^\infty\sin(n\pi x)\brround{A_n\cos(n\pi t)+B_n\sin(n\pi t)}\\
    &v_t(x,t)=\sum_{n=1}^\infty\sin(n\pi x)\brround{-A_nn\pi\sin(n\pi t)+B_nn\pi\cos(n\pi t)}\\
    &v(x,0)=\sum_{n=1}^\infty A_n\sin(n\pi x)=\sin(\pi x)\\
    &A_n=\delta_{1,n}\\
    &v_t(x,0)=\sum_{n=1}B_nn\pi\sin(n\pi x)=\sin(3\pi x)\\
    &B_nn\pi=\delta_{3,n}\Ra B_n=\frac{\delta_{3,n}}{n\pi}\\
    &v(x,t)=\sin(\pi x)\cos(\pi t)+\frac{1}{3\pi}\sin(3\pi x)\sin(3\pi t)\\
    &u(x,t)=x+\sin(\pi x)\cos(\pi t)+\frac{1}{3\pi}\sin(3\pi x)\sin(3\pi t)
\end{align*}
Ex4:
\begin{align*}
    &u_{tt}=c^2u_{xx}+e^{-t}\cos(3x),\ 0<x<\frac{\pi}{2},\ t>0\\
    &u_x(0,t)=0,\ u\brround{\frac{\pi}{2},t}=t\\
    &u(x,0)=\cos x,\ u_t(x,0)=1+\cos(5x)
\end{align*}
Steady state solution:
\begin{align*}
    &u(x,t)=w(x,t)+v(x,t)\\
    &w(x,t)=A(t)x+B(t)\\
    &w_x(x,t)=A(t)\Ra w_x(0,t)=A(t)=0\\
    &w\brround{\frac{\pi}{2},t}=B(t)=t\\
    &w(x,t)=t\\
    &w_{tt}+v_{tt}=c^2w_{xx}+c^2v_{xx}+e^{-t}\cos(3x)\Ra v_{tt}=c^2v_{xx}+e^{-t}\cos(3x)\\
    &w_x(0,t)+v_x(0,t)=0\Ra v_x(0,t)=0\\
    &w\brround{\frac{\pi}{2},t}+v\brround{\frac{\pi}{2},t}=t\Ra v\brround{\frac{\pi}{2},t}=0\\
    &w(x,0)+v(x,0)=v(x,0)=\cos x\\
    &w_t(x,0)+v_t(x,0)=1+v_t(x,0)=1+\cos(5x)\Ra v_t(x,0)=\cos(5x)
\end{align*}
Eigenfunction expansion:\\
Mixed BCs:
\begin{align*}
    &\lambda_n=\brround{\frac{(2n-1)\pi}{2L}}^2=(2n-1)^2\\
    &X_n=\cos(\mu_nx),\ \mu_n=2n-1,\ n\geq1\\
    &v(x,t)=\sum_{n=1}^\infty V_n(t)\cos(\mu_nx)\\
    &S(x,t)=e^{-t}\cos(3x)=\sum_{n=1}^\infty S_n(t)\cos(\mu_n x)\\
    &\mu_n=2n-1=3\Ra n=2\\
    &S_n=e^{-t}\delta_{2,n}\\
    &v_{tt}=\sum_{n=1}^\infty V_n''(t)\cos(\mu_nx)\\
    &v_{xx}=\sum_{n=1}^\infty-V_n(t)\mu_n^2\cos(\mu_nx)\\
    &v_{tt}-c^2v_{xx}-S(x,t)=0\\
    &\sum_{n=1}^\infty\brround{V_n''+c^2\mu_n^2V_n-e^{-t}\delta_{2,n}}\cos(\mu_nx)=0
\end{align*}
2nd Order ODE:
\begin{align*}
    &V_n''+c^2\mu_n^2V_n=\delta_{2,n}e^{-t}\\
    &(V_n)_c=A_n\cos(c\mu_nt)+B_n\sin(c\mu_nt)\\
    &(V_n)_p=C_ne^{-t}= (V_n)_p''\\
    &C_ne^{-t}(1+c^2\mu_n^2)=\delta_{2,n}e^{-t}\\
    &C_n=\frac{\delta_{2,n}}{1+c^2\mu_n^2}\\
    &V_n(t)=A_n\cos(c\mu_nt)+B_n\sin(c\mu_nt)+\frac{\delta_{2,n}e^{-t}}{1+c^2\mu_n^2}
\end{align*}
Impose initial conditions:
\begin{align*}
    &v(x,t)=\sum_{n=1}^\infty\brround{A_n\cos(c\mu_nt)+B_n\sin(c\mu_nt)+\frac{\delta_{2,n}e^{-t}}{1+c^2\mu_n^2}}\cos(\mu_nx)\\
    &v_t(x,t)=\sum_{n=1}^\infty\brround{-A_nc\mu_n\sin(c\mu_nt)+B_nc\mu_n\cos(c\mu_nt)-\frac{\delta_{2,n}e^{-t}}{1+c^2\mu_n^2}}\cos(\mu_nx)\\
    &v(x,0)=\cos x=\sum_{n=1}^\infty\brround{A_n+\frac{\delta_{2,n}}{1+c^2\mu_n^2}}\cos(\mu_nx)\\
    &\mu_n=1=2n-1\Ra n=1\\
    &A_n+\frac{\delta_{2,n}}{1+c^2\mu_n^2}=\delta_{1,n}\Ra A_n=\delta_{1,n}-\frac{\delta_{2,n}}{1+c^2\mu_n^2}\\
    &v_t(x,0)=\cos(5x)=\sum_{n=1}^\infty \brround{B_nc\mu_n-\frac{\delta_{2,n}}{1+c^2\mu_n^2}}\cos(\mu_nx)\\
    &\mu_n=5=2n-1\Ra n=3\\
    &B_nc\mu_n-\frac{\delta_{2,n}}{1+c^2\mu_n^2}=\delta_{3,n}\Ra B_n=\frac{\delta_{3,n}}{c\mu_n}+\frac{\delta_{2,n}}{c\mu_n(1+c^2\mu_n^2)}\\
    &v(x,t)=\cos(ct)\cos(x)+\brround{\frac{e^{-t}-\cos(3ct)}{1+9c^2}+\frac{\sin(3ct)}{3c(1+9c^2)}}\cos(3x)+\frac{\sin(5ct)}{5c}\cos(5x)\\
    &u(x,t)=t+\cos(ct)\cos(x)+\brround{\frac{3ce^{-t}-3c\cos(3ct)+\sin(3ct)}{3c(1+9c^2)}}\cos(3x)+\frac{1}{5c}\sin(5ct)\cos(5x)
\end{align*}

\subsubsection{D'Alembert's Solution}
We can think of the solution to the wave equation as two superimposed waves travelling in opposite directions. This is represented through d'Alembert's solution to the wave equation.\\
Derivation of formula:
\begin{align*}
    &u_{tt}=c^2u_{xx}\\
    &u_{tt}-c^2u_{xx}=0\\
    &(u_t-cu_x)(u_t+cu_x)=0
\end{align*}
We can show that any function of the form $F(x-ct)$ satisfies $u_t+cu_x=0$.
\begin{align*}
    &u(x,t)=F(x-ct)\\
    &\text{let }\xi=x-ct\\
    &u_t=\frac{dF}{d\xi}\frac{d\xi}{dt}=F'(-c)\\
    &u_x=\frac{dF}{d\xi}\frac{d\xi}{dx}=F'(1)\\
    &u_t+cu_x=-cF'+cF'=0
\end{align*}
$\therefore$ $F(x-ct)$ is a solution to $u_t+cu_x=0$\\
Any function $G(x+ct)$ is a solution to $u_t-cu_x=0$
\begin{align*}
    &\text{let }\eta=x+ct\\
    &u_t=\frac{dG}{d\eta}\frac{d\eta}{dt}=G'(c)\\
    &u_x=\frac{dG}{d\eta}\frac{d\eta}{dx}=G'(1)\\
    &\Ra G'(c)-cG'=0
\end{align*}
The solution to $u_{tt}=c^2u_{xx}$ is $u=F(x-ct)+G(x+ct)$.\\
Proving that it's a solution:
\begin{align*}
    &u_{tt}-c^2u_{xx}=0\\
    &u_t=\frac{dF}{d\xi}\frac{d\xi}{dt}+\frac{dG}{d\eta}\frac{d\eta}{dt}\\
    &u_{tt}=\frac{d^2F}{d\xi^2}\cdot c^2+\frac{d^2G}{d\eta^2}\cdot c^2\\
    &u_x=\frac{dF}{d\xi}\frac{d\xi}{dx}+\frac{dF}{d\eta}\frac{d\eta}{dx}\\
    &u_{xx}=\frac{d^2F}{d\xi^2}+\frac{d^2G}{d\eta^2}\\
    &u_{tt}-c^2u_{xx}=F''c^2+G''c^2-c^2(F''+G'')=0\\
    &u(x,t)=F(x-ct)+G(x+ct)\\
    &u(x,0)=f(x)\\
    &u_t(x,0)=g(x)\\
    &u(x,0)=f(x)=F(x)+G(x)\\
    &u_t(x,0)=g(x)=-cF'(x)+cG'(x)\\
    &-cF(x)+cG(x)=\int_0^x g(s)ds\\
    &2cG(x)=\int_0^xg(s)ds+cf(x)\\
    &G(x)=\frac{1}{2c}\int_0^xg(s)ds+\frac{1}{2}f(x)\\
    &2cF(x)=cf(x)-\int_0^x g(s)ds\\
    &\Ra F(x)=\frac{1}{2}f(x)-\frac{1}{2c}\int_0^x g(s)ds\\
    &u(x,t)=F(x-ct)+G(x+ct)\\
    &=\frac{1}{2}f(x-ct)-\frac{1}{2c}\int_0^{x-ct}g(s)ds+\frac{1}{2c}\int_0^{x+ct}g(s)ds+\frac{1}{2}f(x+ct)\\
    &=\frac{1}{2}f(x-ct)+\frac{1}{2}f(x+ct)+\frac{1}{2c}\int_0^{x+ct}g(s)ds+\frac{1}{2c}\int_{x-ct}^0 g(s)ds
\end{align*}
And so the final solution is of the form
$$u(x,t)=\frac{1}{2}\brround{f(x-ct)+f(x+ct)}+\frac{1}{2c}\int_{x-ct}^{x+ct}g(s)ds$$
Ex:
\begin{align*}
    &u_{tt}=u_{xx},\ t>0,\ 0\leq x\leq 1\\
    &u(0,t)=0,\ u(1,t)=1\\
    &u(x,0)=\sin(\pi x)+x,\ u_t(x,0)=\sin(3\pi x)
\end{align*}
D'Alembert's solution:
\begin{small}
\begin{align*}
    &u(x,t)=\frac{1}{2}\brround{f(x-ct)+f(x+ct)}+\frac{1}{2c}\int_{x-ct}^{x+ct}g(s)ds\\
    &u(x,t)=\frac{1}{2}\brround{(x-t)+\sin(\pi(x-t))+(x+t)+\sin(\pi(x+t))+\int_{x-t}^{x+t}\sin(3\pi s)ds}\\
    &=x+\frac{1}{2}\brround{\sin(\pi x)\cos(\pi t)-\cos(\pi x)\sin(\pi t)+\sin(\pi x)\cos(\pi t)+\cos(\pi x)\sin(\pi t)-\frac{1}{3\pi}\brsquare{\cos(3\pi s)}_{x-t}^{x+t}}\\
    &=x+\frac{1}{2}\brround{2\sin(\pi x)\cos(\pi t)-\frac{1}{3\pi}\brround{\cos(3\pi(x+t))-\cos(3\pi(x-t))}}\\
    &=x+\frac{1}{2}\brround{2\sin(\pi x)\cos(\pi t)-\frac{1}{3\pi}\brround{\cos(3\pi x)\cos(3\pi t)-\sin(3\pi x)\sin(3\pi t)-(\cos(3\pi x)\cos(3\pi t)+\sin(3\pi x)\sin(3\pi t))}}\\
    &=x+\frac{1}{2}\brround{2\sin(\pi x)\cos(\pi t)+\frac{2}{3\pi}\sin(3\pi x)\sin(3\pi t)}\\
    &u(x,t)=x+\sin(\pi x)\cos(\pi t)+\frac{1}{3\pi}\sin(3\pi x)\sin(3\pi t)
\end{align*}
\end{small}